fixed abstract spec, refactored most lemmas

src/C_strtoimax/VstProof/AbstractSpec.v
@@ -47,16 +47,19 @@ Section AbstractSpec.
     index : Z ;
   }.
   
-  Fixpoint Z_of_string_loop (s : list byte) (v i : Z) := 
+Definition app_char (b : bool) v c := 
+  if b then  v * 10 + (Z_of_char c) else -v * 10 - (Z_of_char c).
+
+ Fixpoint Z_of_string_loop (s : list byte) (v i : Z) (b : bool) := 
     match s with 
     | [] => {| res := OK ; 
               value := v ; 
               index := i |}
     | c :: tl => 
       if is_digit c
-      then let v1 := v * 10 + (Z_of_char c) in 
+      then let v1 := app_char b v c in 
            if bounded v1
-           then Z_of_string_loop tl v1 (i + 1)
+           then Z_of_string_loop tl v1 (i + 1) b
            else {| res := ERROR_RANGE ;
                    value := v1 ;
                    index := i ; |}      
@@ -64,7 +67,6 @@ Section AbstractSpec.
               value := v ;
               index := i ; |}              
     end.
-
 
   Definition Z_of_string (s : list byte) : Z_of_string_result := 
       match s with 
@@ -75,28 +77,22 @@ Section AbstractSpec.
                 then {| res := EXPECT_MORE ;
                         value := 0 ;
                         index := 1 ; |} 
-                else Z_of_string_loop s 0 0
-      |  ch :: tl => let result := Z_of_string_loop tl 0 1 in
-                    if (Byte.signed ch =? plus_char)
-                    then result
+                else Z_of_string_loop s 0 0 true
+      |  ch :: tl => if (Byte.signed ch =? plus_char)
+                    then  Z_of_string_loop tl 0 1 true
                     else if (Byte.signed ch =? minus_char)
-                         then {| res := res result ;
-                                 value := -1 * (value result) ;
-                                 index := index result ; |}
-                         else Z_of_string_loop s 0 0
+                         then Z_of_string_loop tl 0 1 false
+                         else Z_of_string_loop s 0 0 true
       end.
 
 End AbstractSpec.
 
-Section ClikeSpec.
+Section C_likeSpec.
 
 Definition ASN1_INTMAX_MAX := Int64.max_signed.
 Definition upper_boundary := Z.div ASN1_INTMAX_MAX 10.
 Definition last_digit_max := Zmod ASN1_INTMAX_MAX 10.
 Definition last_digit_max_minus := last_digit_max + 1.
-
-Definition app_char (b : bool) v c := 
-  if b then  v * 10 + (Z_of_char c) else -v * 10 - (Z_of_char c).
 
 Definition last_digit (b : bool) := 
   if b then last_digit_max else last_digit_max_minus.
@@ -109,24 +105,24 @@ Fixpoint Z_of_string_loop_C (s : list byte) (v i : Z) (b : bool):=
     | c :: tl => 
       if is_digit c
       then let d := (Z_of_char c) in 
+           let v1 := v*10 + d in
            if (v <? upper_boundary) 
-           then Z_of_string_loop_C tl (v * 10 + d) (i + 1) b
+           then Z_of_string_loop_C tl v1 (i + 1) b
            else if ((v =? upper_boundary)&&(d <=? (last_digit b)))%bool
-                then let v1 := app_char b v c in
-                     match tl with
+                then match tl with
                      | [] => {| res := OK ; 
                                value := v1 ; 
                                index := (i + 1) |}
                      | c :: tl => if is_digit c
                                  then {| res := ERROR_RANGE ;
-                                         value := v1;
+                                         value := app_char b v1 c;
                                          index := (i + 1) ; |}
                                  else {| res := EXTRA_DATA;
-                                         value := v1 ;
+                                         value := v1;
                                          index := (i + 1) ; |}
                      end
                 else {| res := ERROR_RANGE ;
-                        value := v ;
+                        value := v1 ;
                         index := i ; |}      
       else {| res := EXTRA_DATA ;
               value := v ;
@@ -154,52 +150,11 @@ Definition Z_of_string_C (s : list byte) : Z_of_string_result :=
                     else Z_of_string_loop_C s 0 0 true
   end.
 
-End ClikeSpec.
+End C_likeSpec.
 
-Section AbstractSpec''.
-
- Fixpoint Z_of_string_loop'' (s : list byte) (v i : Z) (b : bool) := 
-    match s with 
-    | [] => {| res := OK ; 
-              value := v ; 
-              index := i |}
-    | c :: tl => 
-      if is_digit c
-      then let v1 := app_char b v c in 
-           if bounded v1
-           then Z_of_string_loop'' tl v1 (i + 1) b
-           else {| res := ERROR_RANGE ;
-                   value := v ;
-                   index := i ; |}      
-      else {| res := EXTRA_DATA ;
-              value := v ;
-              index := i ; |}              
-    end.
-
-
-  Definition Z_of_string'' (s : list byte) : Z_of_string_result := 
-      match s with 
-      |  nil => {| res := ERROR_INVAL ; 
-                  value := 0 ;
-                  index := 0 ; |} 
-      | [ch] => if is_sign ch 
-                then {| res := EXPECT_MORE ;
-                        value := 0 ;
-                        index := 1 ; |} 
-                else Z_of_string_loop'' s 0 0 true
-      |  ch :: tl => if (Byte.signed ch =? plus_char)
-                    then  Z_of_string_loop'' tl 0 1 true
-                    else if (Byte.signed ch =? minus_char)
-                         then Z_of_string_loop'' tl 0 1 false
-                         else Z_of_string_loop'' s 0 0 true
-      end.
-
-End AbstractSpec''.
-
-
+(* alternative abstract spec, with positive loop *)
 Section AbstractSpec'.
 
-  (* true plus, false minus bound *)
   Definition bounded' (b : bool) (n : Z) : bool :=
     if b 
     then andb (0 <=? n) (n <=? Int64.max_signed) 
@@ -213,14 +168,14 @@ Section AbstractSpec'.
     | c :: tl => 
       if is_digit c
       then let v1 := v * 10 + (Z_of_char c) in 
-           if bounded' b v1
+           if bounded' b v
            then Z_of_string_loop' tl v1 (i + 1) b
            else {| res := ERROR_RANGE ;
-                   value := v ;
+                   value := v1 ;
                    index := i ; |}      
       else {| res := EXTRA_DATA ;
               value := v ;
-              index := i ; |}              
+              index := i  ; |}              
     end.
 
 
@@ -246,7 +201,9 @@ Section AbstractSpec'.
 
 End AbstractSpec'.
 
-Lemma aux : forall ls v i, Z_of_string_loop'' ls v i true = 
+(* Correctness of C-like spec *)
+
+Lemma abstract_spec_C_spec_equiv_true : forall ls v i, Z_of_string_loop' ls v i true = 
                       Z_of_string_loop_C ls v i true.
   Proof.
     induction ls.
@@ -261,40 +218,7 @@ Lemma aux : forall ls v i, Z_of_string_loop'' ls v i true =
          simpl.
          bool_rewrite.
          break_if.
-         (* contrdiction *)
-         admit.
-         intuition.
-         simpl.
-         bool_rewrite.
-         intuition.
-      --(* contradiction *)
-        admit.
-      -- (* contradiction *)
-        admit.
-      -- break_match.
-         * (* contradiction *)
-           admit.
-         * (* contradiction *)
-           admit.
-Admitted.
-
-
-Lemma aux' : forall ls v i, Z_of_string_loop' ls v i true = 
-                      Z_of_string_loop_C ls v i true.
-  Proof.
-    induction ls.
-    - intuition.
-    - simpl.
-      intros.
-      repeat break_if;
-        try eapply IHls.
-      break_match.
-      -- intuition.
-      -- break_if.
-         simpl.
-         bool_rewrite.
-         break_if.
-         (* contrdiction *)
+         (* next is out of range *)
          admit.
          intuition.
          simpl.
@@ -304,11 +228,7 @@ Lemma aux' : forall ls v i, Z_of_string_loop' ls v i true =
         admit.
       -- (* contradiction *)
         admit.
-      -- break_match.
-         * (* contradiction *)
-           admit.
-         * (* contradiction *)
-           admit.
+      -- admit.  (* contradiction *)
 Admitted.
 
 Ltac Zbool_to_Prop := try (rewrite Z.leb_le ||
@@ -339,13 +259,70 @@ Proof.
     all: nia.
 Qed.
 
+Lemma abstract_spec_C_spec_equiv_false_res : forall ls v i, 
+    res (Z_of_string_loop' ls v i false) = 
+    res (Z_of_string_loop_C ls v i false).
+Proof.
+ induction ls.
+    - intuition.
+    - simpl.
+      intros.
+      repeat break_if;
+        try eapply IHls.
+      break_match.
+      -- intuition.
+      -- break_if.
+         simpl.
+         bool_rewrite.
+         break_if.
+         (* next is out of range *)
+         admit.
+         intuition.
+         simpl.
+         bool_rewrite.
+         intuition.
+      -- (* contradiction *)
+        admit.
+      -- (* contradiction *)
+        admit.
+      -- admit.  (* contradiction *)
+Admitted.
 
-  Lemma aux_false : forall ls v i, 
-      0 <= v ->
-      0 <= value (Z_of_string_loop' ls v i false) ->
-      value (Z_of_string_loop' ls v i false) = 
-      Z.abs (value (Z_of_string_loop_C ls v i false)).
-  Proof.
+Lemma abstract_spec_C_spec_equiv_false_index : forall ls v i, 
+    index (Z_of_string_loop' ls v i false) = 
+    index (Z_of_string_loop_C ls v i false).
+Proof.
+ induction ls.
+    - intuition.
+    - simpl.
+      intros.
+      repeat break_if;
+        try eapply IHls.
+      break_match.
+      -- intuition.
+      -- break_if.
+         simpl.
+         bool_rewrite.
+         break_if.
+         (* next is out of range *)
+         admit.
+         intuition.
+         simpl.
+         bool_rewrite.
+         intuition.
+      -- (* contradiction *)
+        admit.
+      -- (* contradiction *)
+        admit.
+      -- admit.  (* contradiction *)
+Admitted.
+
+Lemma abstract_spec_C_spec_equiv_false_value : forall ls v i, 
+    0 <= v ->
+    0 <= value (Z_of_string_loop' ls v i false) ->
+    value (Z_of_string_loop' ls v i false) = 
+    Z.abs (value (Z_of_string_loop_C ls v i false)).
+Proof.
     induction ls.
     - simpl.
       intros.
@@ -366,22 +343,18 @@ Qed.
          assert (0 <= v * 10 + Z_of_char a).
          eapply is_digit_to_Z in Heqb.
          nia.
-         replace (- v * 10 - Z_of_char a) with
-           (- (v * 10 + Z_of_char a))
-                 by auto with zarith.
-          Search Z.abs Z.opp.
-          erewrite Z.abs_opp.
-          edestruct  Z.abs_spec with (n :=  v * 10 + Z_of_char a).
-          inversion H2.
-          nia.
-          inversion H2.
-          nia.
+         edestruct  Z.abs_spec with (n :=  v * 10 + Z_of_char a).
+         inversion H2.
+         nia.
+         inversion H2.
+         nia.
       -- break_if.
          simpl.
          bool_rewrite.
          break_if.
-         (* contrdiction *)
+         (* as before *)
          admit.
+         simpl.
          admit.
          simpl.
          bool_rewrite.
@@ -389,11 +362,11 @@ Qed.
           assert (0 <= v * 10 + Z_of_char a).
          eapply is_digit_to_Z in Heqb.
          nia.
-         replace (- v * 10 - Z_of_char a) with
+         (* replace (- v * 10 - Z_of_char a) with
            (- (v * 10 + Z_of_char a))
                  by auto with zarith.
           Search Z.abs Z.opp.
-          erewrite Z.abs_opp.
+          erewrite Z.abs_opp. *)
           edestruct  Z.abs_spec with (n :=  v * 10 + Z_of_char a).
           inversion H2.
           nia.
@@ -420,18 +393,16 @@ Lemma Clike_corr : forall ls, Z_of_string' ls = Z_of_string_C ls.
         replace (value (Z_of_string_loop' (i0 :: l) 0 1 false))
                 with (Z.abs (value (Z_of_string_loop_C (i0 :: l) 0 1 false))).
         admit.
-        erewrite  aux_false.
+        erewrite  abstract_spec_C_spec_equiv_false_value.
         auto.
         nia.
         admit.
-        eapply aux'.
-        erewrite aux_false.
+        eapply  abstract_spec_C_spec_equiv_true.
+        erewrite  abstract_spec_C_spec_equiv_false_value.
         admit.
         nia.
         admit.
         admit.
 Admitted.
-                
 
-      
-  
+
